Formalize up to correctness/completeness thm statements

bolcalc.v
@@ -1,16 +1,35 @@
 (* BOL Derivation Calculus *)
 
+From Coq Require Import ssreflect ssrfun ssrbool.
+Set Implicit Arguments.
+Unset Strict Implicit.
+Unset Printing Implicit Defensive.
+
 Require Import bol.
+Require Import fol.
+Require Import boltofol.
 
 Reserved Notation "Gamma '|-' f" (at level 65).
 
-Definition bolContext := bolFormula -> Prop.
-Definition ctxCons ctx f: bolContext := fun g => (ctx f) \/ f = g.
+Definition context (declType: Type) (formulaType: Type) := ((declType -> Prop) * (formulaType -> Prop))%type.
+Definition bolContext := context bolDecl bolFormula.
 
-Notation "ctx ',' f" := (ctxCons ctx f) (at level 64).
+Definition ctxDeclCons {declType formulaType} ctx d: context declType formulaType := match ctx with
+| (decls, formulae) => (fun e => (decls d) \/ d = e, formulae)
+end.
+
+Definition ctxFormulaCons {declType formulaType} ctx f: context declType formulaType  := match ctx with
+| (decls, formulae) => (decls, fun g => (formulae f) \/ f = g)
+end.
+
+Notation "ctx ',' f" := (ctxFormulaCons ctx f) (at level 64).
+Notation "ctx '+++' f" := (ctxDeclCons ctx f) (at level 64).
+
+Inductive fresh: bolContext -> bolID -> Prop :=.
 
 Inductive bolDerivable : bolContext -> bolFormula -> Prop :=
-  | var: forall (ctx: bolContext) f, ctx f -> ctx |- f
+(*  | var: forall (decls: bolDecl -> Prop) (formulae: bolFormula -> Prop) (ctx: context bolDecl bolFormula) (f: bolFormula),
+      ctx = (decls, formulae) -> formulae f -> ctx |- f*)
   | eq: forall (ctx: bolContext) (F: bolConcept -> bolFormula) c d,
       ctx |- (F c) -> ctx |- c == d -> ctx |- (F d)
 
@@ -53,30 +72,71 @@ Inductive bolDerivable : bolContext -> bolFormula -> Prop :=
 
   | relCompIntro: forall ctx i j k R1 R2,
       ctx |- i <.R1.> j -> ctx |- j <.R2.> k -> ctx |- i <.R1;R2.> k
-  | relCompElim: forall ctx i j k R1 R2 f,    (* TODO j needs to be fresh! *)
+  | relCompElim: forall ctx i j k R1 R2 f,
          ctx |- i <.R1;R2.> k
-      -> ctx, i <.R1.> j, j <.R2.> k |- f
+      -> fresh ctx j
+      -> ctx +++ (IND j), i <.R1.> j, j <.R2.> k |- f
       -> ctx |- f
 
   | relDomIntro: forall ctx i j R,
       ctx |- i <.R.> j -> ctx |- i IS-A (dom R)
-  | relDomElim: forall ctx (i j: bolInd) R f, (* TODO j needs to be fresh! *)
-      ctx |- i IS-A (dom R) -> ctx, (i <.R.> j) |- f -> ctx |- f
+  | relDomElim: forall ctx i j R f,
+        ctx |- i IS-A (dom R)
+     -> fresh ctx j
+     -> ctx +++ IND j, (i <.R.> j) |- f
+     -> ctx |- f
 
   | relCodIntro: forall ctx i j R,
       ctx |- i <.R.> j -> ctx |- j IS-A (cod R)
-  | relCodElim: forall ctx (i j: bolInd) R f, (* TODO i needs to be fresh! *)
-      ctx |- j IS-A (dom R) -> ctx, (i <.R.> j) |- f -> ctx |- f
+  | relCodElim: forall ctx i (j: bolID) R f,
+         ctx |- j IS-A (dom R)
+      -> fresh ctx j
+      -> ctx +++ IND j, (i <.R.> j) |- f
+      -> ctx |- f
 
+  | relForallIntro: forall ctx c R i j,
+         fresh ctx j
+      -> ctx +++ IND j, i <.R.> j |- j IS-A c
+      -> ctx |- j IS-A (c forall R)
   | relForallElim: forall ctx c R i j,
          ctx |- i IS-A (c forall R)
       -> ctx |- i <.R.> j
       -> ctx |- j IS-A c
-  | relExistsElim: forall ctx c R i j f,     (* TODO j needs to be fresh! *)
+
+  | relExistsIntro: forall ctx c R i j,
+         ctx |- i <.R.> j
+      -> ctx |- j IS-A c
+      -> ctx |- i IS-A (c exists R)
+  | relExistsElim: forall ctx c R i j f,
          ctx |- i IS-A (c exists R)
-      -> ctx, i <.R.> j, j IS-A c |- f
+      -> fresh ctx j
+      -> ctx +++ IND j, i <.R.> j, j IS-A c |- f
       -> ctx |- f
 
-  (* missing: forall intro, exists intro *)
-
   where "Gamma '|-' f" := (bolDerivable Gamma f).
+
+Reserved Notation "Gamma '|--' f" (at level 65).
+Definition folContext := context folDecl folFormula.
+Inductive folDerivable : folContext -> folFormula -> Prop :=
+  where "Gamma '|--' f" := (folDerivable Gamma f).
+
+Require Import Coq.Lists.List.
+
+Definition ctxFromSystem {declType folType: Type} (system: (list declType) * (list folType)): context declType folType := match system with
+(* strangely, (sig, thy) pattern matching doesn't work here *)
+| pair sig thy => pair (fun a => False) (fun b => False)
+end.
+
+Notation "'^' sys" := (ctxFromSystem sys) (at level 50).
+Notation "'[[' ontology ']]'" := (bolSemantics ontology) (at level 45).
+
+(* probably true *)
+Theorem correctness: forall (ontology: bolOntology) f,
+  ^ontology |- f -> ^[[ontology]] |-- formulaSemantics f.
+  move => ontology f; elim => //. (* lol due to folDerivable being empty *)
+Qed.
+
+(* probably not true *)
+Theorem completeness: forall (ontology: bolOntology) f,
+  ^[[ontology]] |-- formulaSemantics f -> ^ontology |- f.
+Admitted.
